A bit more progress on paranoid sanity of eqterm.

formalization/ptt.v
@@ -1997,3 +1997,62 @@ Proof.
   destruct (sane_eqterm' G u v A H).
   auto using (@sane_isterm G u A).
 Defined.
+
+Fixpoint TyIdInversion G A u v (H : istype G (Id A u v)) {struct H} :
+  isctx G * istype G A * isterm G u A * isterm G v A.
+Proof.
+  inversion H.
+
+  - { split ; [(split ; [split | idtac]) | idtac].
+
+      - assumption.
+      - apply (@TyCtxConv G0 G) ; auto.
+        now apply TyIdInversion with (u := u) (v := v).
+      - apply (@TermCtxConv G0 G) ; auto.
+        + now apply TyIdInversion with (u := u) (v:= v).
+        + now apply TyIdInversion with (u := u) (v:= v).
+      - apply (@TermCtxConv G0 G) ; auto.
+        + now apply TyIdInversion with (u := u) (v:= v).
+        + now apply TyIdInversion with (u := u) (v:= v).
+    }
+
+  - { split ; [(split ; [split | idtac]) | idtac].
+      - assumption.
+      - assumption.
+      - assumption.
+      - assumption.
+    }
+
+Defined.
+
+Fixpoint ProdTyInversion G A B (H : istype G (Prod A B)) {struct H} :
+  isctx G * istype G A * istype (ctxextend G A) B.
+Proof.
+  inversion H.
+
+  - { split ; [ split | idtac ].
+      - assumption.
+      - apply (@TyCtxConv G0 G) ; auto.
+        now apply (ProdTyInversion G0 A B).
+      - apply (@TyCtxConv (ctxextend G0 A) (ctxextend G A)).
+        + apply CtxExtend ; auto.
+          now apply (ProdTyInversion G0 A B).
+        + apply CtxExtend.
+          * assumption.
+          * apply (@TyCtxConv G0 G) ; auto.
+            now apply (ProdTyInversion G0 A B).
+        + now apply (ProdTyInversion G0 A B).
+        + apply EqCtxExtend ; auto.
+          * now apply (ProdTyInversion G0 A B).
+          * now apply (ProdTyInversion G0 A B).
+          * apply EqTyRefl ; auto.
+            now apply (ProdTyInversion G0 A B).
+    }
+            
+  - { split ; [ split | idtac ].
+      - assumption.
+      - assumption.
+      - assumption.
+    }
+Defined.
+
